
Notes for Flow Matching

Jingxuan Zhang

Department of Computer Science and Engineering
East China University of Science and Technology
Shanghai, China
y21220033@mail.ecust.edu.cn

1 Theory for Basic Flow Matching

According to the Flow Matching paper [1], we need to find a path between the noise distribution $p_0(x_0)$, such as Gaussian, to the data distribution $p_1(x_1)$. To go through the whole path, one possible way is to interpolate the two distributions linearly:

$$x_t = (1 - t)x_0 + tx_1, \quad t \in [0, 1]. \quad (1)$$

Here $x_0 \sim p_0(x_0)$ and $x_1 \sim p_1(x_1)$. Then we can derive the velocity field $v_t(x_t)$ as:

$$v_t(x_t) = \frac{dx_t}{dt} = x_1 - x_0. \quad (2)$$

In the original paper, we use ψ_t to model x and u_t to model the derivative, such as $x_t = \psi_t(x)$ and $\frac{d}{dt}x_t = \frac{d}{dt}\psi_t(x) = u_t(\psi_t(x))$. We construct a neural network $v_t(x_t)$ to approximate the velocity field $u_t(x_t)$. The loss function is defined as:

$$L = \mathbb{E}_{x_t \sim p_t(x_t)} \left[\|v_t(x_t) - u_t(x_t)\|^2 \right]. \quad (3)$$

However, we do not know how to sample from $p_t(x_t)$ nor the ground truth $u_t(x_t)$. To solve this problem, we can represent the loss function as:

$$\begin{aligned} L &= \mathbb{E}_{x_t \sim p_t(x_t)} \left[\|v_t(x_t) - u_t(x_t)\|^2 \right] \\ &= \mathbb{E}_{x_t \sim p_t(x_t)} \left[\|v_t(x_t)\|^2 - 2 \cdot v_t(x_t) \cdot u_t(x_t) + \|u_t(x_t)\|^2 \right] \end{aligned} \quad (4)$$

We first derive the expression of u_t . On the one hand, according to the continuity function:

$$\frac{d}{dt}p_t(x) + \text{div}(p_t(x)u_t(x)) = 0 \quad (5)$$

On the other hand, we have:

$$\begin{aligned} \frac{d}{dt}p_t(x) &= \int \left(\frac{d}{dt}p_t(x|x_1) \right) q(x_1) dx_1 \\ &= - \int \text{div}(u_t(x|x_1)p_t(x|x_1)) q(x_1) dx_1 \\ &= - \text{div} \left(\int (u_t(x|x_1)p_t(x|x_1)) q(x_1) dx_1 \right) \end{aligned} \quad (6)$$

By comparing Eqs. (5) and (6), we have:

$$u_t = \frac{\int u_t(x|x_1)p_t(x|x_1)q(x_1)dx_1}{p_t(x)}. \quad (7)$$

The middle term of Eq. (4) can be transformed using the expectation notation:

$$\begin{aligned}
& \mathbb{E}_{x_t \sim p_t(x)} [2 \cdot v_t(x_t) \cdot u_t(x_t)] = 2 \cdot \int v_t(x_t) \cdot u_t(x_t) \cdot p_t(x_t) dx_t \\
& = 2 \cdot \int v_t(x_t) \cdot \frac{\int u_t(x_t | x_1) p_t(x_t | x_1) q(x_1) dx_1}{p_t(x_t)} \cdot p_t(x_t) dx_t \\
& = 2 \cdot \iint v_t(x_t) \cdot u_t(x_t | x_1) \cdot p_t(x_t | x_1) q(x_1) dx_1 dx_t \\
& = 2 \cdot \mathbb{E}_{x_1 \sim q(x_1), x_t \sim p_t(x_t | x_1)} [v_t(x_t) \cdot u_t(x_t | x_1)]
\end{aligned} \tag{8}$$

After we plug in the above equation, we have:

$$\begin{aligned}
L &= \mathbb{E}_{x_t \sim p_t(x_t)} [\|v_t(x_t)\|^2] - 2 \cdot \mathbb{E}_{x_1 \sim q(x_1), x_t \sim p_t(x_t | x_1)} [v_t(x_t) \cdot u_t(x_t | x_1)] \\
&\quad + \mathbb{E}_{x_t \sim p_t(x_t)} [\|u_t(x_t)\|^2] \\
&= \mathbb{E}_{x_t \sim p_t(x_t)} [\|v_t(x_t)\|^2] - 2 \cdot \mathbb{E}_{x_1 \sim q(x_1), x_t \sim p_t(x_t | x_1)} [v_t(x_t) \cdot u_t(x_t | x_1)] \\
&\quad + \mathbb{E}_{x_t \sim p_t(x_t)} [\|u_t(x_t)\|^2] + \|u_t(x_t | x_1)\|^2 - \|u_t(x_t | x_1)\|^2
\end{aligned} \tag{9}$$

After we swap the last two terms, we have:

$$\begin{aligned}
L &= \mathbb{E}_{x_t \sim p_t(x_t)} [\|v_t(x_t)\|^2] - 2 \cdot \mathbb{E}_{x_1 \sim q(x_1), x_t \sim p_t(x_t | x_1)} [v_t(x_t) \cdot u_t(x_t | x_1)] \\
&\quad + \mathbb{E}_{x_t \sim p_t(x_t)} [\|u_t(x_t | x_1)\|^2] + \mathbb{E}_{x_t \sim p_t(x_t)} [\|u_t(x_t)\|^2 - \|u_t(x_t | x_1)\|^2] \\
&= \mathbb{E}_{x_1 \sim q(x_1), x_t \sim p_t(x_t | x_1)} [\|v_t(x_t)\|^2 - 2 \cdot v_t(x_t) \cdot u_t(x_t | x_1) + \|u_t(x_t | x_1)\|^2] \\
&\quad + \mathbb{E}_{x_t \sim p_t(x_t)} [\|u_t(x_t)\|^2 - \|u_t(x_t | x_1)\|^2] \\
&= \mathbb{E}_{x_1 \sim q(x_1), x_t \sim p_t(x_t | x_1)} [\|v_t(x_t) - u_t(x_t | x_1)\|^2] \\
&\quad + \mathbb{E}_{x_t \sim p_t(x_t)} [\|u_t(x_t)\|^2 - \|u_t(x_t | x_1)\|^2]
\end{aligned} \tag{10}$$

The last term is a constant that does not depend on v_t . Therefore, we can minimize the following loss function instead:

$$L = \mathbb{E}_{x_1 \sim q(x_1), x_t \sim p_t(x_t | x_1)} [\|v_t(x_t) - u_t(x_t | x_1)\|^2]. \tag{11}$$

Suppose $\psi_t(x) = \sigma_t(x_1)x + \mu_t(x_1)$, we have $\psi_t(x_0) = \sigma_t(x_1)x_0 + \mu_t(x_1)$. Let $\mu_t(x_1) = tx_1$, $\sigma_t(x_1) = 1 - t$, then $x_t = \psi_t(x_0) = (1 - t)x_0 + tx_1$, which is the same as our linear interpolation.

Now, remember that $\frac{d}{dt}x_t = \frac{d}{dt}\psi_t(x) = u_t(\psi_t(x))$. We can add a condition to the both sides, and then we have $\frac{d}{dt}\psi_t(x) = u_t(\psi_t(x) | x_1)$ or $\frac{d}{dt}x_t = u_t(x_t | x_1)$ or $\frac{d}{dt}\psi_t(x_0) = u_t(\psi_t(x_0) | x_1)$.

Therefore, the loss function can be rewritten as:

$$L = \mathbb{E}_{x_1 \sim q(x_1), x_0 \sim p_0(x_0)} \left[\left\| v_t(\psi_t(x_0)) - \frac{d}{dt}\psi_t(x_0) \right\|^2 \right]. \tag{12}$$

After calculating the derivative, we have:

$$L = \mathbb{E}_{x_1 \sim q(x_1), x_0 \sim p_0(x_0)} [\|v_t((1 - t)x_0 + tx_1) - (x_1 - x_0)\|^2]. \tag{13}$$

This is the final loss function used in the Flow Matching paper.

References

- [1] Y. Lipman, R. T. Chen, H. Ben-Hamu, M. Nickel, and M. Le, “Flow matching for generative modeling,” in *ICLR*, 2023, pp. 1–28.